
\begin{problem}(1.75 puntos)
Resuelve la siguiente ecuación:

\ppart (0.75) \[x^3-9x = 0\]

\ppart (1) \[
	\frac{(x+2)}{x^3-4x} = \frac{1}{x} - \frac{x^2-x-2}{x^2-2x}
\]
\solution

\spart
\[
	x^3-9x = 0 \dimplies x(x^2-9) = 0 \dimplies x(x+3)(x-3) = 0
\]

\spart 
\[
	\frac{(x+2)}{x^3-4x} = \frac{1}{x} - \frac{(x+1)(x-2)}{x(x-2)} \dimplies
	 \frac{1}{x(x-2)} = \frac{1-(x+1)}{x} \cimplies \frac{1}{x(x-2)} = -1
\]
\[
	\cimplies 1=-x^2+2x \dimplies x^2-2x+1 = 0 \dimplies x_1=x_2=1
\]

\textbf{Comprobación:}

\subparagraph{$x=1$}
\[
\frac{3}{1-4} = \frac{1}{1} - \frac{1-1-2}{1-2} \dimplies \frac{3}{-3} = 1-2 \dimplies -1=-1
\]
Sí es solución.
\end{problem}
